examples/ProcMemCorrect.v
@@ -68,9 +68,11 @@ Section ProcMem.
         * ketrans_r;
             [apply sinModule_duplicate_1;
              [kequiv|kvr|knodup_regs|apply nativeFifoS_const_regs]|].
-          apply duplicate_traceRefines_drop; auto.
-          rewrite <-NativeFifo.nativeFifo_nativeFifoS.
-          apply nfifo_refines_nsfifo.
+          apply duplicate_traceRefines_drop; auto; [kequiv|kvr| |].
+          { vm_compute; tauto. }
+          { rewrite <-NativeFifo.nativeFifo_nativeFifoS.
+            apply nfifo_refines_nsfifo.
+          }
         * apply sinModule_duplicate_1; [kequiv|kvr|knodup_regs|].
           apply nativeFifoS_const_regs with (default:= (getDefaultConst _)).
           
