src/SemFacts.v
@@ -1065,6 +1065,78 @@ Proof.
   apply SubList_app_2, SubList_refl.
 Qed.
 
+Lemma multistep_defs_extDefs_in:
+  forall m (Hequiv: ModEquiv type typeUT m) or ll u,
+    Multistep m or u ll -> Forall (fun l => M.KeysSubset (defs l) (getExtDefs m)) ll.
+Proof.
+  induction ll; intros; auto.
+  inv H; constructor; eauto.
+  eapply step_defs_extDefs_in; eauto.
+Qed.
+
+Lemma multistep_calls_extCalls_in:
+  forall m (Hequiv: ModEquiv type typeUT m) or ll u,
+    Multistep m or u ll -> Forall (fun l => M.KeysSubset (calls l) (getExtCalls m)) ll.
+Proof.
+  induction ll; intros; auto.
+  inv H; constructor; eauto.
+  eapply step_calls_extCalls_in; eauto.
+Qed.
+
+Lemma multistep_defs_ext_in:
+  forall m (Hequiv: ModEquiv type typeUT m) or ll u,
+    Multistep m or u ll -> Forall (fun l => M.KeysSubset (defs l) (getExtMeths m)) ll.
+Proof.
+  induction ll; intros; auto.
+  inv H; constructor; eauto.
+  apply M.KeysSubset_SubList with (d1:= getExtDefs m).
+  - eapply step_defs_extDefs_in; eauto.
+  - apply SubList_app_1, SubList_refl.
+Qed.
+
+Lemma multistep_calls_ext_in:
+  forall m (Hequiv: ModEquiv type typeUT m) or ll u,
+    Multistep m or u ll -> Forall (fun l => M.KeysSubset (calls l) (getExtMeths m)) ll.
+Proof.
+  induction ll; intros; auto.
+  inv H; constructor; eauto.
+  apply M.KeysSubset_SubList with (d1:= getExtCalls m).
+  - eapply step_calls_extCalls_in; eauto.
+  - apply SubList_app_2, SubList_refl.
+Qed.
+
+Lemma behavior_defs_extDefs_in:
+  forall m (Hequiv: ModEquiv type typeUT m) ll u,
+    Behavior m u ll -> Forall (fun l => M.KeysSubset (defs l) (getExtDefs m)) ll.
+Proof.
+  intros; inv H.
+  eapply multistep_defs_extDefs_in; eauto.
+Qed.
+
+Lemma behavior_calls_extCalls_in:
+  forall m (Hequiv: ModEquiv type typeUT m) ll u,
+    Behavior m u ll -> Forall (fun l => M.KeysSubset (calls l) (getExtCalls m)) ll.
+Proof.
+  intros; inv H.
+  eapply multistep_calls_extCalls_in; eauto.
+Qed.
+
+Lemma behavior_defs_ext_in:
+  forall m (Hequiv: ModEquiv type typeUT m) ll u,
+    Behavior m u ll -> Forall (fun l => M.KeysSubset (defs l) (getExtMeths m)) ll.
+Proof.
+  intros; inv H.
+  eapply multistep_defs_ext_in; eauto.
+Qed.
+
+Lemma behavior_calls_ext_in:
+  forall m (Hequiv: ModEquiv type typeUT m) ll u,
+    Behavior m u ll -> Forall (fun l => M.KeysSubset (calls l) (getExtMeths m)) ll.
+Proof.
+  intros; inv H.
+  eapply multistep_calls_ext_in; eauto.
+Qed.
+
 Lemma substepsInd_rule_split:
   forall m o u l,
     SubstepsInd m o u l ->
